More work

src/SDK/Serialize/HeaderV1.dfy
@@ -3,6 +3,7 @@
 
 include "../../../libraries/src/Collections/Sequences/Seq.dfy"
 include "../../Generated/AwsCryptographicMaterialProviders.dfy"
+include "../../AwsCryptographicMaterialProviders/Client.dfy"
 include "../../StandardLibrary/StandardLibrary.dfy"
 include "../../Util/UTF8.dfy"
 include "./SerializableTypes.dfy"
@@ -15,6 +16,7 @@ module HeaderV1 {
   import Aws.Crypto
   import Seq
   import Header
+  import MaterialProviders.Client
   import opened EncryptedDataKeys
   import opened EncryptionContext2
   import opened SerializableTypes
@@ -23,30 +25,75 @@ module HeaderV1 {
   import opened UTF8
   import opened SerializeFunctions
 
-  type V1Header = h: Header.Header
-  | h.body.HeaderBodyV1?
+  type V1HeaderBody = h: Header.HeaderBody
+  | h.HeaderBodyV1?
   witness *
 
   const VERSION_1: seq<uint8> := [0x01];
+  const RESERVED_BYTES: seq<uint8> := [0x00, 0x00, 0x00, 0x00];
 
-  function method WriteHeaderV1(
-    header: V1Header
+  function method WriteHeaderBodyV1(
+    body: V1HeaderBody
   ):
     (ret: seq<uint8>)
   {
-    var connonicalEC := CanonicalEncryptionContext(header.body.encryptionContext);
+    var connonicalEC := CanonicalEncryptionContext(body.encryptionContext);
+    var suiteId := GetAlgorithmSuiteId(body.esdkSuiteId);
+    var suite := Client.SpecificationClient().GetSuite(suiteId);
 
     VERSION_1
-    + header.body.messageType.Serialize()
-    + UInt16ToSeq(header.body.esdkSuiteId)
-    + header.body.messageId
+    + [body.messageType.Serialize()]
+    + UInt16ToSeq(body.esdkSuiteId)
+    + body.messageId
     + WriteAADSection(connonicalEC)
-    + WriteEncryptedDataKeys(header.body.encryptedDataKeys)
-    + [header.body.contentType.Serialize()]
-    + [0x00, 0x00, 0x00, 0x00]
-    + UInt32ToSeq(header.body.frameLength)
-    + header.body.suiteData
+    + WriteEncryptedDataKeys(body.encryptedDataKeys)
+    + [body.contentType.Serialize()]
+    + RESERVED_BYTES
+    + [suite.encrypt.ivLength]
+    + UInt32ToSeq(body.frameLength)
   }
 
+  function method ReadHeaderBodyV1(
+    s: seq<uint8>,
+    pos: nat
+  ):
+    (res: ReadCorrect<V1HeaderBody>)
+    ensures CorrectlyRead(s, pos, res, WriteHeaderBodyV1)
+  {
+    var (version, messageTypeStart) :- SerializeFunctions.Read(s, pos, 1);
+
+    :- Need(version == VERSION_1, Error("Incorrect message version."));
+    var (messageTypeByte, suiteStart) :- Read(s, messageTypeStart, 1);
+    var messageType :- Header.MessageType.Get(messageTypeByte[0]).MapFailure(e => Error(e));
+    var (esdkSuiteId, messageIdStart) :- ReadUInt16(s, suiteStart);
+    :- Need(esdkSuiteId in VALID_IDS, Error("Algorithm suite not supported."));
+    var suiteId := GetAlgorithmSuiteId(esdkSuiteId);
+    var suite := Client.SpecificationClient().GetSuite(suiteId);
+    var (messageId, ecStart) :- Read(s, messageIdStart, Header.MESSAGE_ID_LEN);
+    var (canonicalEncryptionContext, edkStart) :- EncryptionContext2.ReadAADSection(s, ecStart);
+    var encryptionContext: ESDKEncryptionContext := EncryptionContext2.EncryptionContext(canonicalEncryptionContext);
+    var (encryptedDataKeys, contentTypeStart) :- EncryptedDataKeys.ReadEncryptedDataKeysSection(s, edkStart);
+    var (contentTypeByte, reservedStart) :- Read(s, contentTypeStart, 1);
+    var contentType :- Header.ContentType.Get(contentTypeByte[0]).MapFailure(e => Error(e));
+    var (reservedBytes, headerIvLengthStart) :- Read(s, reservedStart, 4);
+    :- Need(RESERVED_BYTES == reservedBytes, Error("Invalid Reserved Bytes"));
+    var (headerIvLengthByte, frameLengthStart) :- Read(s, headerIvLengthStart, 1);
+    var headerIvLength := headerIvLengthByte[0];
+    :- Need(headerIvLength == suite.encrypt.ivLength, Error("Invalid IVLength."));
+    var (frameLength, end) :- ReadUInt32(s, frameLengthStart);
+
+    var body:V1HeaderBody := Header.HeaderBodyV1(
+      messageType := messageType,
+      esdkSuiteId := esdkSuiteId,
+      messageId := messageId,
+      encryptionContext := encryptionContext,
+      encryptedDataKeys := encryptedDataKeys,
+      contentType := contentType,
+      headerIvLength := headerIvLength as nat,
+      frameLength := frameLength
+    );
+
+    Success((body, end))
+  }
 
 }
